dump.v
@@ -376,3 +376,140 @@ Admitted.
   assert (ARITY (CO F Gs) < arity (convert (CO F Gs))).
   { apply ARITY_le_arity. apply strict_cons with (G:=G). easy. }
   lia.
+
+
+Lemma list_max_ge : ∀ l n, In n l → n ≤ list_max l.
+Proof.
+  intros. induction l.
+  - false.
+  - simpl in *. destruct H.
+    + subst. lia.
+    + apply Nat.max_le_iff. right. apply IHl. easy.
+Qed.
+
+Open Scope nat.
+Lemma strict_cons : ∀ F G Gs, strict (CO F (G :: Gs)) → strict (CO F Gs).
+Proof.
+  intros. inverts H.
+  apply strCO.
+  - easy.
+  - apply Forall_inv_tail in H3. easy.
+  - simpl in H4. lia.
+  - apply Forall_inv_tail in H5.
+    destruct Gs.
+    + simpl. easy.
+    + assert (ARITY (CO F (G :: p :: Gs)) = ARITY (CO F (p :: Gs))).
+      { simpl. assert (H6 := H5).
+        apply Forall_inv in H5. apply Forall_inv_tail in H6.
+        simpl in *. lia. }
+      rewrite H in H5. easy.
+Qed.
+
+Lemma arity_co_cons : ∀ F G Gs, Gs ≠ [] → strict (CO F (G::Gs)) →
+  ARITY (CO F Gs) = ARITY (CO F (G::Gs)).
+Proof.
+  intros. assert (H1 := strict_cons H0). inverts H0. inverts H1.
+  destruct Gs. false.
+  apply Forall_inv_tail in H7. apply Forall_inv in H7.
+  apply Forall_inv in H10. lia.
+Qed.
+
+Lemma anc_co_lt1 : ∀ F G Gs, strict (CO F (G :: Gs)) →
+  anc (CO F Gs) < anc (CO F (G :: Gs)).
+Admitted.
+
+Lemma anc_co_lt2 : ∀ F G Gs, strict (CO F (G :: Gs)) →
+  anc G < anc (CO F (G :: Gs)).
+Admitted.
+
+Open Scope Z.
+Goal ∀ F Gs l n,
+  Forall (λ G, strict G) Gs →
+  Forall (λ G, ARITY G = ARITY (CO F Gs)) Gs →
+  Forall (λ G, thesis G l 0) Gs →
+  ARITY (CO F Gs) = length l →
+  anc (CO F Gs) ≤ n →
+  «co_loading (ARITY (CO F Gs)) (map convert Gs)»
+    (↑↑l ++ repeat 0%Z n) =
+  ↑↑map (λ G, EVALUATE G l) Gs ++ ↑↑l ++ repeat 0%Z (n - length Gs).
+Proof.
+  intros. gen l n. induction Gs.
+  - intros. simpl. autorewrite with arith_base. reflexivity.
+  - intros. simpl co_loading. segment.
+    assert (list_max (map ARITY Gs) ≤ ARITY a).
+    { apply Forall_inv in H0.
+      rewrite H0. simpl. lia. }
+    simpl in H2. rewrite max_l in *.
+    pose (anc_co_lt1 F a Gs). pose (anc_co_lt2 F a Gs).
+    asserts_rewrite (
+      « \ [ARITY a] \ » (↑↑ l ++ repeat 0 n) =
+      0 :: ↑↑l ++ repeat 0 (n-1) ).
+    { unfold perm. simpl call_list. rewrite Nat.add_0_r.
+      rewrite call_def.
+      replace ((↑↑ l ++ repeat 0 n) ^[ ARITY a])
+      with [0].
+      replace ((↑↑ l ++ repeat 0 n) ^[ 0, ARITY a])
+      with (↑↑l).
+      replace ((↑↑l ++ repeat 0 n) ^[ 1 + ARITY a, ∞ ])
+      with (repeat 0 (n-1)).
+      reflexivity.
+      rewrite skipn_app. rewrite skipn_all2. rewrite app_nil_l.
+      rewrite repeat_skipn. f_equal. f_equal. rewrite map_length.
+      lia. rewrite map_length. lia.
+      rewrite splice_app. rewrite splice_all. rewrite splice_gt.
+      rewrite app_nil_r. reflexivity.
+      rewrite map_length. lia. rewrite map_length. lia.
+      rewrite splice_app. rewrite splice_all2. rewrite app_nil_l.
+      rewrite map_length.
+      replace (1 + ARITY a - length l)%nat with (1+(ARITY a - length l))%nat.
+      replace (ARITY a - length l)%nat with O.
+      rewrite splice_nth with (d:=0). f_equal.
+      generalize (anc (CO F (a :: Gs))). intros.
+      destruct n. reflexivity. reflexivity.
+      rewrite repeat_length.
+      lia. lia. lia. rewrite map_length. lia.
+      rewrite app_length. rewrite map_length.
+      rewrite repeat_length. lia. }
+    rewrite thesis_le.
+    rewrite pa_def. simpl. f_equal.
+    destruct Gs. reflexivity.
+    assert (ARITY a = ARITY p).
+    { pose (Forall_inv H0) as H5. simpl in H5.
+      pose (Forall_inv_tail H0) as H6.
+      apply Forall_inv in H6. simpl in H6.
+      lia. }
+    assert (ARITY (CO F (p::Gs)) = ARITY a).
+    { rewrite H5. apply Forall_inv_tail in H0.
+      apply Forall_inv in H0. rewrite H0. simpl. lia. }
+    remember (p::Gs) as Gs'.
+    rewrite <- H6.
+    replace (n - S (length Gs'))%nat with ((n - 1) - length Gs')%nat.
+    apply IHGs.
+    apply Forall_inv_tail in H. easy.
+    apply Forall_inv_tail in H0.
+    assert (ARITY (CO F Gs') = ARITY (CO F (a::Gs'))).
+    { simpl in *. lia. } rewrite H7. apply H0.
+    apply Forall_inv_tail in H1. easy.
+    lia. lia. lia.
+    apply Forall_inv in H1. easy.
+    lia.
+    apply Forall_inv in H. easy.
+    easy. easy. easy.
+Qed.
+
+
+apply Forall_inv_tail in H8.
+        apply Forall_inv in H8. rewrite H8. simpl. lia.
+
+
+      rewrite repeat_spec with (n:=anc (CO F (a :: Gs)))(x:=0).
+      reflexivity. apply nth_in_or_default.
+      generalize (repeat 0 (anc (CO F (a :: Gs)))). intros.
+      destruct l0. reflexivity. simpl.
+
+rewrite max_l.
+
+  x + ↑(EVALUATE F l) :: ↑↑l ++ repeat 0 (anc F).
+
+
+Admitted.
